feat(library/init/data/array/basic): add `Array.extract`

library/init/data/array/basic.lean
@@ -18,7 +18,7 @@ structure Array (α : Type u) :=
 
 attribute [extern cpp inline "lean::array_sz(#2)"] Array.sz
 
-@[extern cpp inline "lean::array_get_size(#2)"]
+@[reducible, extern cpp inline "lean::array_get_size(#2)"]
 def Array.size {α : Type u} (a : @& Array α) : Nat :=
 a.sz
 
@@ -28,7 +28,7 @@ variables {α : Type u} {β : Type v}
 /- The parameter `c` is the initial capacity -/
 @[extern cpp inline "lean::mk_empty_array(#2)"]
 def mkEmpty (c : @& Nat) : Array α :=
-{ sz   := 0,
+{ sz := 0,
   data := λ ⟨x, h⟩, absurd h (Nat.notLtZero x) }
 
 @[extern cpp inline "lean::array_push(#2, #3)"]
@@ -62,26 +62,26 @@ def singleton (v : α) : Array α :=
 mkArray 1 v
 
 @[extern cpp inline "lean::array_index(#2, #3)"]
-def index (a : @& Array α) (i : @& Fin a.sz) : α :=
+def index (a : @& Array α) (i : @& Fin a.size) : α :=
 a.data i
 
 /- Low-level version of `index` which is as fast as a C array read.
    `Fin` values are represented as tag pointers in the Lean runtime. Thus,
    `index` may be slightly slower than `idx`. -/
 @[extern cpp inline "lean::array_idx(#2, #3)"]
-def idx (a : @& Array α) (i : USize) (h : i.toNat < a.sz) : α :=
+def idx (a : @& Array α) (i : USize) (h : i.toNat < a.size) : α :=
 a.index ⟨i.toNat, h⟩
 
 /- "Comfortable" version of `index`. It performs a bound check at runtime. -/
 @[extern cpp inline "lean::array_get(#2, #3, #4)"]
 def get [Inhabited α] (a : @& Array α) (i : @& Nat) : α :=
-if h : i < a.sz then a.index ⟨i, h⟩ else default α
+if h : i < a.size then a.index ⟨i, h⟩ else default α
 
 def getOpt (a : Array α) (i : Nat) : Option α :=
 if h : i < a.size then some (a.index ⟨i, h⟩) else none
 
 @[extern cpp inline "lean::array_update(#2, #3, #4)"]
-def update (a : Array α) (i : @& Fin a.sz) (v : α) : Array α :=
+def update (a : Array α) (i : @& Fin a.size) (v : α) : Array α :=
 { sz   := a.sz,
   data := λ j, if h : i = j then v else a.data j }
 
@@ -89,20 +89,20 @@ def update (a : Array α) (i : @& Fin a.sz) (v : α) : Array α :=
    `Fin` values are represented as tag pointers in the Lean runtime. Thus,
    `update` may be slightly slower than `updt`. -/
 @[extern cpp inline "lean::array_updt(#2, #3, #4)"]
-def updt (a : Array α) (i : USize) (v : α) (h : i.toNat < a.sz) : Array α :=
+def updt (a : Array α) (i : USize) (v : α) (h : i.toNat < a.size) : Array α :=
 a.update ⟨i.toNat, h⟩ v
 
 /- "Comfortable" version of `update`. It performs a bound check at runtime. -/
 @[extern cpp inline "lean::array_set(#2, #3, #4)"]
 def set (a : Array α) (i : @& Nat) (v : α) : Array α :=
-if h : i < a.sz then a.update ⟨i, h⟩ v else a
+if h : i < a.size then a.update ⟨i, h⟩ v else a
 
-theorem szUpdateEq (a : Array α) (i : Fin a.sz) (v : α) : (update a i v).sz = a.sz :=
+theorem szUpdateEq (a : Array α) (i : Fin a.size) (v : α) : (update a i v).size = a.size :=
 rfl
 
 @[extern cpp inline "lean::array_pop(#2)"]
 def pop (a : Array α) : Array α :=
-{ sz   := Nat.pred a.sz,
+{ sz   := Nat.pred a.size,
   data := λ ⟨j, h⟩, a.index ⟨j, Nat.ltOfLtOfLe h (Nat.predLe _)⟩ }
 
 -- TODO(Leo): justify termination using wf-rec
@@ -114,14 +114,14 @@ variables {m : Type v → Type v} [Monad m]
 local attribute [instance] monadInhabited'
 
 -- TODO(Leo): justify termination using wf-rec
-@[specialize] partial def miterateAux (a : Array α) (f : Π i : Fin a.sz, α → β → m β) : Nat → β → m β
+@[specialize] partial def miterateAux (a : Array α) (f : Π i : Fin a.size, α → β → m β) : Nat → β → m β
 | i b :=
-  if h : i < a.sz then
-     let idx : Fin a.sz := ⟨i, h⟩ in
+  if h : i < a.size then
+     let idx : Fin a.size := ⟨i, h⟩ in
      f idx (a.index idx) b >>= miterateAux (i+1)
   else pure b
 
-@[inline] def miterate (a : Array α) (b : β) (f : Π i : Fin a.sz, α → β → m β) : m β :=
+@[inline] def miterate (a : Array α) (b : β) (f : Π i : Fin a.size, α → β → m β) : m β :=
 miterateAux a f 0 b
 
 @[inline] def mfoldl (a : Array α) (b : β) (f : α → β → m β) : m β :=
@@ -135,8 +135,8 @@ local attribute [instance] monadInhabited
 -- TODO(Leo): justify termination using wf-rec
 @[specialize] partial def mfindAux (a : Array α) (f : α → m (Option β)) : Nat → m (Option β)
 | i :=
-  if h : i < a.sz then
-     let idx : Fin a.sz := ⟨i, h⟩ in
+  if h : i < a.size then
+     let idx : Fin a.size := ⟨i, h⟩ in
      do r ← f (a.index idx),
         (match r with
          | some v := pure r
@@ -148,7 +148,7 @@ mfindAux a f 0
 
 end
 
-@[inline] def iterate (a : Array α) (b : β) (f : Π i : Fin a.sz, α → β → β) : β :=
+@[inline] def iterate (a : Array α) (b : β) (f : Π i : Fin a.size, α → β → β) : β :=
 Id.run $ miterateAux a f 0 b
 
 @[inline] def foldl (a : Array α) (f : α → β → β) (b : β) : β :=
@@ -160,13 +160,13 @@ Id.run $ mfoldlFrom a b f ini
 @[inline] def find (a : Array α) (f : α → Option β) : Option β :=
 Id.run $ mfindAux a f 0
 
-@[specialize] private def revIterateAux (a : Array α) (f : Π i : Fin a.sz, α → β → β) : Π (i : Nat), i ≤ a.sz → β → β
+@[specialize] private def revIterateAux (a : Array α) (f : Π i : Fin a.size, α → β → β) : Π (i : Nat), i ≤ a.size → β → β
 | 0     h b := b
 | (j+1) h b :=
-  let i : Fin a.sz := ⟨j, h⟩ in
+  let i : Fin a.size := ⟨j, h⟩ in
   revIterateAux j (Nat.leOfLt h) (f i (a.index i) b)
 
-@[inline] def revIterate (a : Array α) (b : β) (f : Π i : Fin a.sz, α → β → β) : β :=
+@[inline] def revIterate (a : Array α) (b : β) (f : Π i : Fin a.size, α → β → β) : β :=
 revIterateAux a f a.size (Nat.leRefl _) b
 
 @[inline] def revFoldl (a : Array α) (b : β) (f : α → β → β) : β :=
@@ -184,23 +184,23 @@ instance [HasToString α] : HasToString (Array α) :=
 section
 variables {m : Type u → Type u} [Monad m]
 
-@[inline] private def mforeachAux (a : Array α) (f : Π i : Fin a.sz, α → m α) : m { a' : Array α // a'.sz = a.sz } :=
+@[inline] private def mforeachAux (a : Array α) (f : Π i : Fin a.size, α → m α) : m { a' : Array α // a'.size = a.size } :=
 miterate a ⟨a, rfl⟩ $ λ i v ⟨a', h⟩, do
-  let i' : Fin a'.sz := Eq.recOn h.symm i,
+  let i' : Fin a'.size := Eq.recOn h.symm i,
   x ← f i v,
   pure $ ⟨a'.update i' x, (szUpdateEq a' i' x) ▸ h⟩
 
-@[inline] def mforeach (a : Array α) (f : Π i : Fin a.sz, α → m α) : m (Array α) :=
+@[inline] def mforeach (a : Array α) (f : Π i : Fin a.size, α → m α) : m (Array α) :=
 Subtype.val <$> mforeachAux a f
 
 @[inline] def mmap (f : α → m α) (a : Array α) : m (Array α) :=
 mforeach a (λ _, f)
 end
 
-@[inline] def foreach (a : Array α) (f : Π i : Fin a.sz, α → α) : Array α :=
+@[inline] def foreach (a : Array α) (f : Π i : Fin a.size, α → α) : Array α :=
 Id.run $ mforeach a f
 
-theorem szForeachEq (a : Array α) (f : Π i : Fin a.sz, α → α) : (foreach a f).sz = a.sz :=
+theorem szForeachEq (a : Array α) (f : Π i : Fin a.size, α → α) : (foreach a f).size = a.size :=
 (Id.run $ mforeachAux a f).property
 
 /- Homogeneous map -/
@@ -213,7 +213,20 @@ then foreach a (λ ⟨i, h'⟩, f (b.index ⟨i, Nat.ltOfLtOfLe h' h⟩))
 else foreach b (λ ⟨i, h'⟩, f (a.index ⟨i, Nat.ltTrans h' (Nat.gtOfNotLe h)⟩))
 
 def map (f : α → β) (as : Array α) : Array β :=
-as.foldl (λ a bs, bs.push (f a)) (mkEmpty as.sz)
+as.foldl (λ a bs, bs.push (f a)) (mkEmpty as.size)
+
+-- TODO(Leo): justify termination using wf-rec
+partial def extractAux (a : Array α) : Nat → Π (e : Nat), e ≤ a.size → Array α → Array α
+| i e hle r :=
+  if hlt : i < e then
+    let idx : Fin a.size := ⟨i, Nat.ltOfLtOfLe hlt hle⟩ in
+    extractAux (i+1) e hle (r.push (a.index idx))
+ else r
+
+def extract (a : Array α) (b e : Nat) : Array α :=
+let r : Array α := mkEmpty (e - b) in
+if h : e ≤ a.size then extractAux a b e h r
+else r
 
 end Array
 
